Finish optimization lectures.

src/opt.v
@@ -1,7 +1,17 @@
 From stdpp Require Import base gmap ssreflect strings.
 From introduction Require Import imp.
 
-Definition cp_add e1 e2 :=
+(** With the semantics of Imp in place, we can define a _constant folding_
+    optimization that removes intermediate computations that are known to be
+    constant.  Let us begin with expressions.  Given a binary operation [b], we
+    define a function that computes an optimized version of [b] with constant
+    folding. If no optimization applies, we keep the operation as is.
+
+    For example, we optimize addition as follows. We combine literals by adding
+    them together.  If one of the terms is zero, we keep the other one, even if
+    it is not constant -- after all, adding zero should not change anything.  *)
+
+Definition cf_add e1 e2 :=
   match e1, e2 with
   | Num n1, Num n2 => Num (n1 + n2)
   | Num 0, e
@@ -9,7 +19,32 @@ Definition cp_add e1 e2 :=
   | _, _ => Binop Add e1 e2
   end.
 
-Definition cp_mul e1 e2 :=
+(** The key property of [cf_add] is that it does not change the result of
+    evaluation. *)
+
+Lemma cf_add_correct : forall e1 e2 s,
+  eval_expr (cf_add e1 e2) s
+  = eval_expr (Binop Add e1 e2) s.
+(* <admitted> *)
+Proof.
+intros e1 e2 s.
+destruct e1 as [x1|[|n1]|b1 e11 e12];
+destruct e2 as [x2|[|n2]|b2 e21 e22];
+rewrite /=; eauto.
+- destruct (s !! x1) as [n1|]; rewrite /=; eauto.
+- destruct (s !! x2) as [n2|]; rewrite /=; eauto.
+- destruct (eval_expr e21 s) as [n21| |]; rewrite /=; eauto.
+  destruct (eval_expr e22 s) as [n22| |]; rewrite /=; eauto.
+- destruct (eval_expr e11 s) as [n11| |]; rewrite /=; eauto.
+  destruct (eval_expr e12 s) as [n12| |]; rewrite /=; eauto.
+Qed.
+(* </admitted> *)
+
+(* <skip /> *)
+
+(** Let's try another operation: multiplication. *)
+
+Definition cf_mul e1 e2 :=
   match e1, e2 with
   | Num n1, Num n2 => Num (n1 * n2)
   | Num 0, _
@@ -19,159 +54,55 @@ Definition cp_mul e1 e2 :=
   | _, _ => Binop Mul e1 e2
   end.
 
-Definition cp_sub e1 e2 :=
-  match e1, e2 with
-  | Num n1, Num n2 => Num (n1 - n2)
-  | Num 0, _ => Num 0
-  | _, Num 0 => e1
-  | _, _ => Binop Sub e1 e2
-  end.
+(* <skip /> *)
 
-Definition cp_leq e1 e2 :=
-  match e1, e2 with
-  | Num n1, Num n2 => Num (eval_binop Leq n1 n2)
-  | Num 0, _ => Num 1
-  | _, _ => Binop Leq e1 e2
-  end.
-
-Definition cp_binop b :=
-  match b with
-  | Add => cp_add
-  | Mul => cp_mul
-  | Sub => cp_sub
-  | Leq => cp_leq
-  end.
-
-Fixpoint cp_expr e :=
-  match e with
-  | Binop b e1 e2 => cp_binop b (cp_expr e1) (cp_expr e2)
-  | _ => e
-  end.
-
-Definition cp_seq c1 c2 :=
-  match c1, c2 with
-  | Skip, c
-  | c, Skip => c
-  | _, _ => Seq c1 c2
-  end.
-
-Definition cp_assign x e :=
-  match e with
-  | Var y => if bool_decide (x = y) then Skip else Assign x e
-  | _ => Assign x e
-  end.
-
-Definition cp_if e c1 c2 :=
-  if bool_decide (c1 = c2) then c1
-  else match e with
-       | Num n => if bool_decide (n = 0) then c2 else c1
-       | _ => If e c1 c2
-       end.
-
-Definition cp_while e c :=
-  if bool_decide (e = Num 0) then Skip else While e c.
-
-Fixpoint cp_com c :=
-  match c with
-  | Skip => Skip
-  | Seq c1 c2 => cp_seq (cp_com c1) (cp_com c2)
-  | Assign x e => cp_assign x (cp_expr e)
-  | If e c1 c2 => cp_if (cp_expr e) (cp_com c1) (cp_com c2)
-  | While e c => cp_while (cp_expr e) (cp_com c)
-  end.
-
-Definition cp_add_spec (e1 e2 e : expr) : Prop :=
-  (exists n1 n2, e1 = Num n1 /\ e2 = Num n2 /\ e = Num (n1 + n2)) \/
-  (e1 = Num 0 /\ e2 = e) \/
-  (e1 = e /\ e2 = Num 0) \/
-  (e = Binop Add e1 e2).
-
-Lemma cp_addP e1 e2 : cp_add_spec e1 e2 (cp_add e1 e2).
+Lemma cf_mul_correct : forall e1 e2 s,
+  eval_expr (cf_mul e1 e2) s
+  = eval_expr (Binop Mul e1 e2) s.
 Proof.
-rewrite /cp_add_spec.
-destruct e1 as [x1|[|n1]|b1 e11 e12];
-destruct e2 as [x2|[|n2]|b2 e21 e22];
-eauto 10.
-Qed.
+intros e1 e2 s.
+destruct e1 as [x1|n1|b1 e11 e12];
+destruct e2 as [x2|n2|b2 e21 e22];
+rewrite /=; eauto.
+- (* e1 = Var x1; e2 = Num n2 *)
+  destruct n2 as [|n2]; rewrite /=; eauto.
+  + (* n2 = 0 *)
+    destruct (s !! x1) as [n1|]; rewrite /=; eauto.
+    (* s !! x1 = Some n1 |- Done 0 = Error *)
+    (* Oops... *)
+Abort.
 
-Definition cp_mul_spec (e1 e2 e : expr) : Prop :=
-  (exists n1 n2, e1 = Num n1 /\ e2 = Num n2 /\ e = Num (n1 * n2)) \/
-  (e1 = Num 0 /\ e = Num 0) \/
-  (e2 = Num 0 /\ e = Num 0) \/
-  (e1 = Num 1 /\ e2 = e) \/
-  (e1 = e /\ e2 = Num 1) \/
-  (e = Binop Mul e1 e2).
+(** It turns out that the goal is not provable! What went wrong? If the
+    expression is of the form [e1 * 0], the optimizer replaces it with [0]. The
+    issue is that evaluating [e1] can return an error, whereas evaluating just
+    [0] cannot.  Therefore, optimization can turn an errorneous execution into a
+    successful one, thus modifying the behavior of the program.
 
-Lemma cp_mulP e1 e2 : cp_mul_spec e1 e2 (cp_mul e1 e2).
-Proof.
-rewrite /cp_mul_spec.
-destruct e1 as [x1|[|[|n1]]|b1 e11 e12]; eauto;
-destruct e2 as [x2|[|[|n2]]|b2 e21 e22]; eauto 10.
-Qed.
+    What can we do? We have a few possibilities:
 
-Definition cp_sub_spec e1 e2 e : Prop :=
-  (exists n1 n2, e1 = Num n1 /\ e2 = Num n2 /\ e = Num (n1 - n2)) \/
-  (e1 = Num 0 /\ e = Num 0) \/
-  (e1 = e /\ e2 = Num 0) \/
-  (e = Binop Sub e1 e2).
+    1. Include a side condition to describe when the equation holds. We might:
 
-Lemma cp_subP e1 e2 : cp_sub_spec e1 e2 (cp_sub e1 e2).
-Proof.
-rewrite /cp_sub_spec.
-destruct e1 as [x1|[|n1]|b1 e11 e12]; eauto;
-destruct e2 as [x2|[|n2]|b2 e21 e22]; eauto 10.
-Qed.
+       a. Use a _static_ side condition that can be evaluated during compilation
+          or linking. For example, we might require that all required variables
+          are defined in the initial memory (cf. last lecture).
 
-Definition cp_leq_spec e1 e2 e : Prop :=
-  (exists n1 n2, e1 = Num n1 /\ e2 = Num n2 /\
-                 e = Num (eval_binop Leq n1 n2)) \/
-  (e1 = Num 0 /\ e = Num 1) \/
-  (e = Binop Leq e1 e2).
+       b. Use a _dynamic_ side condition that depends on the particular behavior
+          of the program on the state [s]. For example, we might not require
+          anything if the original program yields an error on [s].
 
-Lemma cp_leqP e1 e2 : cp_leq_spec e1 e2 (cp_leq e1 e2).
-Proof.
-rewrite /cp_leq_spec.
-destruct e1 as [x1|[|n1]|b1 e11 e12]; eauto;
-destruct e2 as [x2|[|n2]|b2 e21 e22]; eauto 10.
-Qed.
+    2. Change the optimization function to make the theorem true.
 
-Definition cp_seq_spec c1 c2 c : Prop :=
-  (c1 = Skip /\ c2 = c) \/
-  (c1 = c /\ c2 = Skip) \/
-  (c = Seq c1 c2).
-
-Lemma cp_seqP c1 c2 : cp_seq_spec c1 c2 (cp_seq c1 c2).
-Proof.
-rewrite /cp_seq_spec.
-destruct c1; destruct c2; eauto 10.
-Qed.
-
-Definition cp_assign_spec x e c :=
-  (e = Var x /\ c = Skip) \/
-  (e <> Var x /\ c = Assign x e).
-
-Lemma cp_assignP x e : cp_assign_spec x e (cp_assign x e).
-Proof.
-rewrite /cp_assign_spec.
-destruct e as [y|n|b e1 e2]; eauto 10.
-rewrite /= bool_decide_decide.
-destruct (decide (x = y)) as [->|?]; eauto.
-assert (Var y ≠ Var x) as ?. { congruence. }
-eauto.
-Qed.
-
-Definition cp_if_spec e c1 c2 c :=
-  (c1 = c2 /\ c2 = c) \/
-  (e = Num 0 /\ c2 = c) \/
-  (exists n, e = Num n /\ n <> 0 /\ c1 = c) \/
-  (c = If e c1 c2).
-
-Lemma cp_ifP e c1 c2 : cp_if_spec e c1 c2 (cp_if e c1 c2).
-Proof.
-rewrite /cp_if_spec /cp_if.
-destruct (bool_decide_reflect (c1 = c2)) as [<-|_]; eauto 10.
-destruct e as [x|[|n]|*]; eauto 10.
-Qed.
+    Option (2) is OK, but limiting: it rules out some optimizations that we
+    would like to do.  Option (1.a) is popular with strongly typed languages,
+    where we can be analyze the required side conditions ahead of time.  Option
+    (1.b) is popular with weakly typed or unsafe languages like C, where it is
+    just too difficult to rule out the problematic cases statically.  For
+    example, if our language had dynamically allocated arrays of variable size,
+    it would be very difficult to guarantee ahead of time that every memory
+    access is safe.  We are going to go with option (1.b), stated in a slightly
+    more convenient form.  The relation [improves r1 r2] says that the behavior
+    of the computation [r1] improves the behavior of the computation [r2], in
+    the sense that it exhibits fewer errors. *)
 
 Definition improves {T} (x y : result T) : Prop :=
   y = Error \/ x = y.
@@ -187,6 +118,25 @@ Hint Resolve improves_error improves_refl : core.
 Lemma improves_trans {T} (x y z : result T) :
   improves x y -> improves y z -> improves x z.
 Proof. by move=> H1 [->|<-]. Qed.
+
+(** This definition makes [Error] a form of _undefined behavior_. In unsafe
+    languages like C, the language implementation is allowed to do anything with
+    the generated code if the source code exhibits undefined behavior, such as
+    accessing undefined memory.  Option (1.a) interprets errors as _unobservable
+    behavior_: they are guaranteed not to occur during execution.  Option (2)
+    interprets errors as undesirable, but legitimate behaviors.  For example, a
+    dynamic type error in a safe language such as JavaScript leads to a run-time
+    exception that can be caught and handled, leading to a non-erroneous
+    outcome. These different interpretations lead to trade-offs in language
+    design involving expressiveness, performance and safety.
+
+    (Notice that this definition forces us to preserve [NotYet], and, thus,
+    preserve non-terminatation. We could have adopted a more lax approach where
+    non-termination can be improved or where timing behavior is not preserved,
+    but we will not pursue this idea here.)
+
+    We will follow the steps of the last lecture and prove some lemmas for
+    reasoning about [improves] compositionally.  The second *)
 
 Lemma improves_bind {T S} (x y : result T) (f g : T -> result S) :
   improves x y ->
@@ -205,26 +155,82 @@ assert (H := eval_expr_notyet e s).
 destruct eval_expr; rewrite /=; done.
 Qed.
 
-Lemma cp_add_correct e1 e2 s :
-  eval_expr (cp_add e1 e2) s = eval_expr (Binop Add e1 e2) s.
-Proof.
-destruct (cp_addP e1 e2) as [H|[H|[H|H]]].
-- destruct H as (n1 & n2 & -> & -> & ->). done.
-- destruct H as (-> & <-). rewrite /=.
-  destruct eval_expr; eauto.
-- destruct H as (<- & ->). rewrite /=.
-  destruct eval_expr; eauto; rewrite /=.
-  rewrite Nat.add_0_r. done.
-- rewrite H. done.
-Qed.
+(** Let's now prove that [cf_mul] is correct. *)
 
-Lemma cp_mul_correct e1 e2 s :
+Lemma cf_mul_correct : forall e1 e2 s,
   improves
-    (eval_expr (cp_mul e1 e2) s)
+    (eval_expr (cf_mul e1 e2) s)
     (eval_expr (Binop Mul e1 e2) s).
+(* <admitted> *)
 Proof.
 rewrite /=.
-destruct (cp_mulP e1 e2) as [H|[H|[H|[H|[H|H]]]]].
+intros e1 e2 s.
+destruct e1 as [x1|n1|b1 e11 e12];
+destruct e2 as [x2|n2|b2 e21 e22];
+rewrite /=; eauto.
+- (* e1 = Var x1; e2 = Num n2 *)
+  destruct n2 as [|[|n2]]; rewrite /=; eauto.
+  + (* n2 = 0 *)
+    destruct (s !! x1) as [n1|]; rewrite /=; eauto.
+    rewrite Nat.mul_0_r. done.
+  + (* n2 = 1 *)
+    destruct (s !! x1) as [n1|]; rewrite /=; eauto.
+    rewrite Nat.mul_1_r. done.
+- (* e1 = Num n1; e2 = Var x2 *)
+  destruct n1 as [|[|n1]]; rewrite /=; eauto.
+  + (* n1 = 0 *)
+    destruct (s !! x2) as [n2|]; rewrite /=; eauto.
+  + (* n1 = 1 *)
+    destruct (s !! x2) as [n2|]; rewrite /=; eauto.
+    rewrite Nat.add_0_r. done.
+- (* e1 = Num n1; e2 = Num n2
+     boring... *)
+Abort.
+(* </admitted> *)
+(* <exercise-only>Reset cf_mul_correct.</exercise-only> *)
+
+(** We could complete this proof, but it is getting tedious. One reason is the
+    branching structure.  The definition of [cf_mul] has six branches; however,
+    Rocq does not have a primitive notion of complex, nested pattern matching.
+    Such match expressions are compiled to a chain of nested matches, which can
+    lead to more nested branches than we might realize.  We can see this in the
+    above proof: to analyze the possible shapes of [e1] and [e2], we need to
+    look at nine subcases, and some of them require further case analysis.
+
+    One possible solution is to use proof automation to avoid considering all
+    these subcases explicitlty.  We are going to follow a lighterweight, more
+    direct approach: we'll define a custom case analysis principle for [cf_mul]
+    that follows the structure of the definition.  Thus, we'll only have to
+    consider the branches that are given in the definition of [cf_mul]
+    itself. *)
+
+Definition cf_mul_spec (e1 e2 e : expr) : Prop :=
+  (exists n1 n2, e1 = Num n1 /\ e2 = Num n2 /\ e = Num (n1 * n2)) \/
+  (e1 = Num 0 /\ e = Num 0) \/
+  (e2 = Num 0 /\ e = Num 0) \/
+  (e1 = Num 1 /\ e2 = e) \/
+  (e1 = e /\ e2 = Num 1) \/
+  (e = Binop Mul e1 e2).
+
+Lemma cf_mulP e1 e2 : cf_mul_spec e1 e2 (cf_mul e1 e2).
+Proof.
+rewrite /cf_mul_spec.
+destruct e1 as [x1|[|[|n1]]|b1 e11 e12]; eauto;
+destruct e2 as [x2|[|[|n2]]|b2 e21 e22]; eauto 10.
+Qed.
+
+(** The lemma [cf_mulP] tells us how the result [cf_mul e1 e2] depends on the
+    expressions [e1] and [e2], depending on which branch of the definition was
+    used.  This allows us to improve our proof as follows. *)
+
+Lemma cf_mul_correct : forall e1 e2 s,
+  improves
+    (eval_expr (cf_mul e1 e2) s)
+    (eval_expr (Binop Mul e1 e2) s).
+(* <admitted> *)
+Proof.
+intros e1 e2 s.
+destruct (cf_mulP e1 e2) as [H|[H|[H|[H|[H|H]]]]].
 - destruct H as (n1 & n2 & -> & -> & ->). done.
 - destruct H as (-> & ->). rewrite /=.
   apply improves_eval_expr. done.
@@ -239,12 +245,63 @@ destruct (cp_mulP e1 e2) as [H|[H|[H|[H|[H|H]]]]].
   apply improves_bind; eauto; intros n. rewrite /= Nat.mul_1_r. done.
 - rewrite H. done.
 Qed.
+(* </admitted> *)
 
-Lemma cp_sub_correct e1 e2 s :
-  improves (eval_expr (cp_sub e1 e2) s) (eval_expr (Binop Sub e1 e2) s).
+(** We are going to follow a similar approach for the remaining optimization
+    steps.  Here is how we can optimize [Sub] and [Leq].  Notice that, just like
+    the case for multiplication, some of the branches simply ignore what the
+    other expression is doing.  (Remember that, since we are working with
+    natural numbers, subtraction is weird: it is truncated at 0.) *)
+
+Definition cf_sub e1 e2 :=
+  match e1, e2 with
+  | Num n1, Num n2 => Num (n1 - n2)
+  | Num 0, _ => Num 0
+  | _, Num 0 => e1
+  | _, _ => Binop Sub e1 e2
+  end.
+
+Definition cf_leq e1 e2 :=
+  match e1, e2 with
+  | Num n1, Num n2 => Num (eval_binop Leq n1 n2)
+  | Num 0, _ => Num 1
+  | _, _ => Binop Leq e1 e2
+  end.
+
+Definition cf_binop b :=
+  match b with
+  | Add => cf_add
+  | Mul => cf_mul
+  | Sub => cf_sub
+  | Leq => cf_leq
+  end.
+
+Definition cf_sub_spec (e1 e2 e : expr) : Prop :=
+(* <exercise-only>(* Replace this *) False.</exercise-only> *)
+(* <solution> *)
+  (exists n1 n2, e1 = Num n1 /\ e2 = Num n2 /\ e = Num (n1 - n2)) \/
+  (e1 = Num 0 /\ e = Num 0) \/
+  (e1 = e /\ e2 = Num 0) \/
+  (e = Binop Sub e1 e2).
+(* </solution> *)
+
+Lemma cf_subP e1 e2 : cf_sub_spec e1 e2 (cf_sub e1 e2).
+(* <commented> *)
 Proof.
-rewrite /=.
-destruct (cp_subP e1 e2) as [H|[H|[H|H]]].
+rewrite /cf_sub_spec.
+destruct e1 as [x1|[|n1]|b1 e11 e12]; eauto;
+destruct e2 as [x2|[|n2]|b2 e21 e22]; eauto 10.
+Qed.
+(* </commented> *)
+(* <exercise-only>Proof. Admitted.</exercise-only> *)
+
+Lemma cf_sub_correct : forall e1 e2 s,
+  improves (eval_expr (cf_sub e1 e2) s)
+    (eval_expr (Binop Sub e1 e2) s).
+(* <admitted> *)
+Proof.
+intros e1 e2 s. rewrite /=.
+destruct (cf_subP e1 e2) as [H|[H|[H|H]]].
 - destruct H as (n1 & n2 & -> & -> & ->). done.
 - destruct H as (-> & ->). rewrite /=.
   by apply: improves_eval_expr => ?; rewrite Nat.sub_0_l.
@@ -253,62 +310,230 @@ destruct (cp_subP e1 e2) as [H|[H|[H|H]]].
   by apply: improves_bind => // n; rewrite Nat.sub_0_r.
 - rewrite H. done.
 Qed.
+(* </admitted> *)
 
-Lemma cp_leq_correct e1 e2 s :
-  improves (eval_expr (cp_leq e1 e2) s) (eval_expr (Binop Leq e1 e2) s).
+Definition cf_leq_spec (e1 e2 e : expr) : Prop :=
+(* <exercise-only>(* Replace this *) False.</exercise-only> *)
+(* <solution> *)
+  (exists n1 n2, e1 = Num n1 /\ e2 = Num n2 /\
+                 e = Num (eval_binop Leq n1 n2)) \/
+  (e1 = Num 0 /\ e = Num 1) \/
+  (e = Binop Leq e1 e2).
+(* </solution> *)
+
+Lemma cf_leqP e1 e2 : cf_leq_spec e1 e2 (cf_leq e1 e2).
+(* <commented> *)
 Proof.
-rewrite /=.
-destruct (cp_leqP e1 e2) as [H|[H|H]].
+rewrite /cf_leq_spec.
+destruct e1 as [x1|[|n1]|b1 e11 e12]; eauto;
+destruct e2 as [x2|[|n2]|b2 e21 e22]; eauto 10.
+Qed.
+(* </commented> *)
+(* <exercise-only>Proof. Admitted.</exercise-only> *)
+
+Lemma cf_leq_correct : forall e1 e2 s,
+  improves (eval_expr (cf_leq e1 e2) s)
+    (eval_expr (Binop Leq e1 e2) s).
+(* <admitted> *)
+Proof.
+intros e1 e2 s. rewrite /=.
+destruct (cf_leqP e1 e2) as [H|[H|H]].
 - destruct H as (n1 & n2 & -> & -> & ->). done.
 - destruct H as (-> & ->). rewrite /=.
   by apply: improves_eval_expr.
 - by rewrite H.
 Qed.
+(* </admitted> *)
 
-Lemma cp_binop_correct s b e1 e2 :
-  improves (eval_expr (cp_binop b e1 e2) s) (eval_expr (Binop b e1 e2) s).
+Lemma cf_binop_correct : forall b e1 e2 s,
+  improves (eval_expr (cf_binop b e1 e2) s)
+    (eval_expr (Binop b e1 e2) s).
 Proof.
-destruct b.
-- by rewrite cp_add_correct.
-- apply cp_mul_correct.
-- apply cp_sub_correct.
-- apply cp_leq_correct.
+intros b e1 e2 s. destruct b.
+- rewrite cf_add_correct. done.
+- apply cf_mul_correct.
+- apply cf_sub_correct.
+- apply cf_leq_correct.
 Qed.
 
-Lemma cp_expr_correct e s :
-  improves (eval_expr (cp_expr e) s) (eval_expr e s).
+(** Now that we can simplify a single binary operation, we can compose such
+    optimizations to handle entire expressions. *)
+
+Fixpoint cf_expr (e : expr) : expr :=
+(* <exercise-only>(* Replace this *) Num 0.</exercise-only> *)
+(* <solution> *)
+  match e with
+  | Binop b e1 e2 => cf_binop b (cf_expr e1) (cf_expr e2)
+  | _ => e
+  end.
+(* </solution> *)
+
+Lemma cf_expr_correct : forall e s,
+  improves (eval_expr (cf_expr e) s) (eval_expr e s).
+(* <admitted> *)
 Proof.
-induction e as [x|n'|b e1 IH1 e2 IH2]; eauto.
-eapply improves_trans. { eapply cp_binop_correct. }
+intros e s. induction e as [x|n'|b e1 IH1 e2 IH2]; eauto.
+eapply improves_trans. { eapply cf_binop_correct. }
 rewrite /=.
 apply improves_bind; eauto. intros n1.
 apply improves_bind; eauto.
 Qed.
-Hint Resolve cp_expr_correct : core.
+(* </admitted> *)
+Hint Resolve cf_expr_correct : core.
 
-Lemma cp_seq_correct c1 c2 k s :
-  improves (eval_com (cp_seq c1 c2) k s) (eval_com (Seq c1 c2) k s).
+(** We can follow the same approach to optimize commands.  We define what it
+    means to optimize each syntactic form, prove the correctness of each
+    optimization step, and then compose everything. *)
+
+Definition cf_seq (c1 c2 : com) : com :=
+(* <exercise-only>(* Replace this *) Skip.</exercise-only> *)
+(* <solution> *)
+  match c1, c2 with
+  | Skip, c
+  | c, Skip => c
+  | _, _ => Seq c1 c2
+  end.
+(* </solution> *)
+
+Definition cf_assign (x : string) (e : expr) : com :=
+(* <exercise-only>(* Replace this *) Skip.</exercise-only> *)
+(* <solution> *)
+  match e with
+  | Var y => if bool_decide (x = y) then Skip else Assign x e
+  | _ => Assign x e
+  end.
+(* </solution> *)
+
+Definition cf_if (e : expr) (c1 c2 : com) : com :=
+(* <exercise-only>(* Replace this *) Skip.</exercise-only> *)
+(* <solution> *)
+  if bool_decide (c1 = c2) then c1
+  else match e with
+       | Num n => if bool_decide (n = 0) then c2 else c1
+       | _ => If e c1 c2
+       end.
+(* </solution> *)
+
+Definition cf_while (e : expr) (c : com) : com :=
+(* <exercise-only>(* Replace this *) Skip.</exercise-only> *)
+(* <solution> *)
+  if bool_decide (e = Num 0) then Skip else While e c.
+(* </solution> *)
+
+Fixpoint cf_com c :=
+  match c with
+  | Skip => Skip
+  | Seq c1 c2 => cf_seq (cf_com c1) (cf_com c2)
+  | Assign x e => cf_assign x (cf_expr e)
+  | If e c1 c2 => cf_if (cf_expr e) (cf_com c1) (cf_com c2)
+  | While e c => cf_while (cf_expr e) (cf_com c)
+  end.
+
+(** We use the same trick as before to prove the correctness of each
+    optimization. We prove a specification to allow us to structure the proof of
+    correctness following the definition of each optimization. *)
+
+Definition cf_seq_spec (c1 c2 c : com) : Prop :=
+(* <exercise-only>(* Replace this *) False.</exercise-only> *)
+(* <solution> *)
+  (c1 = Skip /\ c2 = c) \/
+  (c1 = c /\ c2 = Skip) \/
+  (c = Seq c1 c2).
+(* </solution> *)
+
+Lemma cf_seqP c1 c2 : cf_seq_spec c1 c2 (cf_seq c1 c2).
+(* <commented> *)
 Proof.
-destruct (cp_seqP c1 c2) as [H|[H|H]]; rewrite /=.
+rewrite /cf_seq_spec.
+destruct c1; destruct c2; eauto 10.
+Qed.
+(* </commented> *)
+(* <exercise-only>Proof. Admitted.</exercise-only> *)
+
+Definition cf_assign_spec (x : string) (e : expr) (c : com) : Prop :=
+(* <exercise-only>(* Replace this *) False.</exercise-only> *)
+(* <solution> *)
+  (e = Var x /\ c = Skip) \/
+  (c = Assign x e).
+(* </solution> *)
+
+Lemma cf_assignP x e : cf_assign_spec x e (cf_assign x e).
+(* <commented> *)
+Proof.
+rewrite /cf_assign_spec /cf_assign.
+destruct e as [y|n|b e1 e2]; eauto 10;
+rewrite /= bool_decide_decide.
+destruct (decide (x = y)) as [->|?]; eauto.
+Qed.
+(* </commented> *)
+(* <exercise-only>Proof. Admitted.</exercise-only> *)
+
+Definition cf_if_spec (e : expr) (c1 c2 c : com) : Prop :=
+(* <exercise-only>(* Replace this *) False.</exercise-only> *)
+(* <solution> *)
+  (c1 = c2 /\ c2 = c) \/
+  (e = Num 0 /\ c2 = c) \/
+  (exists n, e = Num n /\ n <> 0 /\ c1 = c) \/
+  (c = If e c1 c2).
+(* </solution> *)
+
+Lemma cf_ifP e c1 c2 : cf_if_spec e c1 c2 (cf_if e c1 c2).
+(* <commented> *)
+Proof.
+rewrite /cf_if_spec /cf_if.
+destruct (bool_decide_reflect (c1 = c2)) as [<-|_]; eauto 10.
+destruct e as [x|[|n]|???]; eauto 10.
+Qed.
+(* </commented> *)
+(* <exercise-only>Proof. Admitted.</exercise-only> *)
+
+Definition cf_while_spec (e : expr) (c c' : com) : Prop :=
+(* <exercise-only>(* Replace this *) False.</exercise-only> *)
+(* <solution> *)
+  (e = Num 0 /\ c' = Skip) \/
+  c' = While e c.
+(* </solution> *)
+
+Lemma cf_whileP e c : cf_while_spec e c (cf_while e c).
+(* <commented> *)
+Proof.
+rewrite /cf_while /cf_while_spec.
+destruct bool_decide eqn:E; eauto.
+rewrite bool_decide_eq_true in E. rewrite E /=; eauto.
+Qed.
+(* </commented> *)
+(* <exercise-only>Proof. Admitted.</exercise-only> *)
+
+Lemma cf_seq_correct : forall c1 c2 k s,
+  improves (eval_com (cf_seq c1 c2) k s) (eval_com (Seq c1 c2) k s).
+(* <admitted> *)
+Proof.
+intros c1 c2 k s.
+destruct (cf_seqP c1 c2) as [H|[H|H]]; rewrite /=.
 - destruct H as (-> & <-). done.
 - destruct H as (<- & ->). rewrite result_mbind_done. done.
 - rewrite H. done.
 Qed.
+(* </admitted> *)
 
-Lemma cp_assign_correct x e k s :
-  improves (eval_com (cp_assign x e) k s) (eval_com (Assign x e) k s).
+Lemma cf_assign_correct : forall x e k s,
+  improves (eval_com (cf_assign x e) k s) (eval_com (Assign x e) k s).
+(* <admitted> *)
 Proof.
-destruct (cp_assignP x e) as [H|H].
+intros x e k s. destruct (cf_assignP x e) as [H|H].
 - destruct H as (-> & ->). rewrite /=.
   destruct (s !! x) as [n|] eqn:E; rewrite /=; eauto.
   rewrite insert_id; done.
-- destruct H as (_ & ->). done.
+- rewrite H. done.
 Qed.
+(* </admitted> *)
 
-Lemma cp_if_correct e c1 c2 k s :
-  improves (eval_com (cp_if e c1 c2) k s) (eval_com (If e c1 c2) k s).
+Lemma cf_if_correct : forall e c1 c2 k s,
+  improves (eval_com (cf_if e c1 c2) k s) (eval_com (If e c1 c2) k s).
+(* <admitted> *)
 Proof.
-destruct (cp_ifP e c1 c2) as [H|[H|[H|H]]]; rewrite /=.
+intros e c1 c2 k s.
+destruct (cf_ifP e c1 c2) as [H|[H|[H|H]]]; rewrite /=.
 - destruct H as (<- & <-).
   apply improves_eval_expr. intros n.
   destruct bool_decide; done.
@@ -317,16 +542,22 @@ destruct (cp_ifP e c1 c2) as [H|[H|[H|H]]]; rewrite /=.
   rewrite bool_decide_eq_false_2; done.
 - rewrite H. done.
 Qed.
+(* </admitted> *)
 
-Lemma cp_while_correct e c k s :
-  improves (eval_com (cp_while e c) k s) (eval_com (While e c) k s).
+Lemma cf_while_correct : forall e c k s,
+  improves (eval_com (cf_while e c) k s) (eval_com (While e c) k s).
+(* <admitted> *)
 Proof.
-rewrite /cp_while.
-destruct bool_decide eqn:E.
-- rewrite bool_decide_eq_true in E. rewrite E /=.
-  destruct k; done.
-- done.
+intros e c k s.
+destruct (cf_whileP e c) as [H| ->]; eauto.
+destruct H as [-> ->]. rewrite /=.
+destruct k; done.
 Qed.
+(* </admitted> *)
+
+(** We conclude by chaining together all of these local correctness results.  We
+    use the following auxiliary lemma, which guarantees that iteration is
+    compatible with improvement. *)
 
 Lemma iter_improves {T} (f g : (T -> result T) -> T -> result T) x k :
   (∀ f' g', (∀ x, improves (f' x) (g' x)) ->
@@ -337,20 +568,29 @@ intros H.
 induction k as [|k IH] in x |- *; rewrite /=; apply H; eauto.
 Qed.
 
-Lemma cp_com_correct c k s :
-  improves (eval_com (cp_com c) k s) (eval_com c k s).
+Lemma cf_com_correct : forall c k s,
+  improves (eval_com (cf_com c) k s) (eval_com c k s).
+(* <admitted> *)
 Proof.
+intros c k s.
 induction c as [|c1 IH1 c2 IH2|x e|e c1 IH1 c2 IH2|e c IH] in s, k |- *.
 - done.
-- rewrite /=. eapply improves_trans. { eapply cp_seq_correct. }
+- rewrite /=. eapply improves_trans. { eapply cf_seq_correct. }
   rewrite /=. apply improves_bind; eauto.
-- rewrite /=. eapply improves_trans. { eapply cp_assign_correct. }
+- rewrite /=. eapply improves_trans. { eapply cf_assign_correct. }
   rewrite /=. apply improves_bind; eauto.
-- rewrite /=. eapply improves_trans. { eapply cp_if_correct. }
+- rewrite /=. eapply improves_trans. { eapply cf_if_correct. }
   rewrite /=. apply improves_bind; eauto. intros n.
   destruct bool_decide; eauto.
-- rewrite /=. eapply improves_trans. { eapply cp_while_correct. }
+- rewrite /=. eapply improves_trans. { eapply cf_while_correct. }
   rewrite /=. apply iter_improves. intros f g f_g s'.
   apply improves_bind; eauto. intros [|n]; rewrite /=; eauto.
   apply improves_bind; eauto.
 Qed.
+(* </admitted> *)
+
+(** Exercise: Define a _constant propagation_ pass, which inlines the values of
+    variables when they are known to be constant.  One possibility is to
+    parameterize the optimization functions by a value [m : gmap string nat]
+    which maps each variable to a natural number that is guaranteed to be its
+    value during execution.  Prove that your definition is correct. *)
